src/coq/Handlers/UndefinedBehaviour.v
@@ -1,8 +1,34 @@
 From Vellvm Require Import
+     PropT
      LLVMEvents.
 
 From ITree Require Import
      ITree.
 
-Definition UB_handler: forall {X}, UBE X -> (itree void1 X -> Prop) := fun _ _ _ => True.
+From ExtLib Require Import
+     Structures.Monads.
+
+Set Implicit Arguments.
+Set Contextual Implicit.
+
+Import MonadNotation.
+Open Scope monad_scope.
+
+Definition UB_handler {E}: UBE ~> PropT (itree E) := fun _ _ _ => True.
+
+Section PARAMS.
+  Variable (E F: Type -> Type).
+
+  Definition E_trigger_prop : E ~> PropT (itree (E +' F)) :=
+    fun R e => fun t => t = r <- trigger e ;; ret r.
+
+  Definition F_trigger_prop : F ~> PropT (itree (E +' F)) :=
+    fun R e => fun t => t = r <- trigger e ;; ret r.
+
+  Definition model_UB :
+    PropT (itree (E +' UBE +' F)) ~> PropT (itree (E +' F)) :=
+    fun T Pt t =>
+      exists t', Pt t' /\ interp_prop (case_ E_trigger_prop (case_ UB_handler F_trigger_prop)) _ t' t.
+
+End PARAMS.
 
